coq/SMT/Simplification.v
@@ -100,6 +100,10 @@ Definition normalize_binop_bv32 op (ast1 ast2 : smt_ast Sort_BV32) :=
   end
 .
 
+Definition normalize_binop_bv40 op (ast1 ast2 : smt_ast Sort_BV40) :=
+  AST_BinOp Sort_BV40 op ast1 ast2
+.
+
 Definition normalize_binop_bv48 op (ast1 ast2 : smt_ast Sort_BV48) :=
   AST_BinOp Sort_BV48 op ast1 ast2
 .
@@ -121,6 +125,7 @@ Definition normalize_binop op (s : smt_sort) (ast1 ast2 : smt_ast s) : smt_ast s
     | Sort_BV16 => normalize_binop_bv16
     | Sort_BV24 => normalize_binop_bv24
     | Sort_BV32 => normalize_binop_bv32
+    | Sort_BV40 => normalize_binop_bv40
     | Sort_BV48 => normalize_binop_bv48
     | Sort_BV56 => normalize_binop_bv56
     | Sort_BV64 => normalize_binop_bv64
@@ -199,6 +204,11 @@ Definition normalize_cmpop_bv32 op (ast1 ast2 : smt_ast Sort_BV32) : smt_ast Sor
   | _ => AST_CmpOp Sort_BV32 op ast1 ast2
   end
 .
+
+Definition normalize_cmpop_bv40 op (ast1 ast2 : smt_ast Sort_BV40) : smt_ast Sort_BV1 :=
+  AST_CmpOp Sort_BV40 op ast1 ast2
+.
+
 Definition normalize_cmpop_bv48 op (ast1 ast2 : smt_ast Sort_BV48) : smt_ast Sort_BV1 :=
   AST_CmpOp Sort_BV48 op ast1 ast2
 .
@@ -245,6 +255,7 @@ Definition normalize_cmpop op (s : smt_sort) (ast1 ast2 : smt_ast s) : smt_ast S
     | Sort_BV16 => normalize_cmpop_bv16
     | Sort_BV24 => normalize_cmpop_bv24
     | Sort_BV32 => normalize_cmpop_bv32
+    | Sort_BV40 => normalize_cmpop_bv40
     | Sort_BV48 => normalize_cmpop_bv48
     | Sort_BV56 => normalize_cmpop_bv56
     | Sort_BV64 => normalize_cmpop_bv64
@@ -261,6 +272,7 @@ Definition normalize_not (s : smt_sort) (ast : smt_ast s) : smt_ast s :=
     | Sort_BV16 => AST_Not Sort_BV16
     | Sort_BV24 => AST_Not Sort_BV24
     | Sort_BV32 => AST_Not Sort_BV32
+    | Sort_BV40 => AST_Not Sort_BV40
     | Sort_BV48 => AST_Not Sort_BV48
     | Sort_BV56 => AST_Not Sort_BV56
     | Sort_BV64 => AST_Not Sort_BV64
@@ -323,6 +335,10 @@ Definition normalize_ite_bv32 cond (ast1 ast2 : smt_ast Sort_BV32) :=
   AST_ITE Sort_BV32 cond ast1 ast2
 .
 
+Definition normalize_ite_bv40 cond (ast1 ast2 : smt_ast Sort_BV40) :=
+  AST_ITE Sort_BV40 cond ast1 ast2
+.
+
 Definition normalize_ite_bv48 cond (ast1 ast2 : smt_ast Sort_BV48) :=
   AST_ITE Sort_BV48 cond ast1 ast2
 .
@@ -343,6 +359,7 @@ Definition normalize_ite (s : smt_sort) cond (ast1 ast2 : smt_ast s) : smt_ast s
     | Sort_BV16 => normalize_ite_bv16
     | Sort_BV24 => normalize_ite_bv24
     | Sort_BV32 => normalize_ite_bv32
+    | Sort_BV40 => normalize_ite_bv40
     | Sort_BV48 => normalize_ite_bv48
     | Sort_BV56 => normalize_ite_bv56
     | Sort_BV64 => normalize_ite_bv64
@@ -447,6 +464,10 @@ Definition simplify_binop_bv32 op (ast1 ast2 : smt_ast Sort_BV32) :=
   end
 .
 
+Definition simplify_binop_bv40 op (ast1 ast2 : smt_ast Sort_BV40) :=
+  AST_BinOp Sort_BV40 op ast1 ast2
+.
+
 Definition simplify_binop_bv48 op (ast1 ast2 : smt_ast Sort_BV48) :=
   AST_BinOp Sort_BV48 op ast1 ast2
 .
@@ -467,6 +488,7 @@ Definition simplify_binop op (s : smt_sort) (ast1 ast2 : smt_ast s) : smt_ast s 
     | Sort_BV16 => simplify_binop_bv16
     | Sort_BV24 => simplify_binop_bv24
     | Sort_BV32 => simplify_binop_bv32
+    | Sort_BV40 => simplify_binop_bv40
     | Sort_BV48 => simplify_binop_bv48
     | Sort_BV56 => simplify_binop_bv56
     | Sort_BV64 => simplify_binop_bv64
@@ -526,6 +548,10 @@ Definition simplify_cmpop_bv32 op (ast1 ast2 : smt_ast Sort_BV32) :=
   end
 .
 
+Definition simplify_cmpop_bv40 op (ast1 ast2 : smt_ast Sort_BV40) :=
+  AST_CmpOp Sort_BV40 op ast1 ast2
+.
+
 Definition simplify_cmpop_bv48 op (ast1 ast2 : smt_ast Sort_BV48) :=
   AST_CmpOp Sort_BV48 op ast1 ast2
 .
@@ -557,6 +583,7 @@ Definition simplify_cmpop op (s : smt_sort) (ast1 ast2 : smt_ast s) : smt_ast So
     | Sort_BV16 => simplify_cmpop_bv16
     | Sort_BV24 => simplify_cmpop_bv24
     | Sort_BV32 => simplify_cmpop_bv32
+    | Sort_BV40 => simplify_cmpop_bv40
     | Sort_BV48 => simplify_cmpop_bv48
     | Sort_BV56 => simplify_cmpop_bv56
     | Sort_BV64 => simplify_cmpop_bv64
@@ -634,6 +661,7 @@ Proof.
   { apply Int16.add_commut. }
   { apply Int24.add_commut. }
   { apply Int32.add_commut. }
+  { apply Int40.add_commut. }
   { apply Int48.add_commut. }
   { apply Int56.add_commut. }
   { apply Int64.add_commut. }
@@ -712,6 +740,7 @@ Proof.
   { apply Int16.mul_commut. }
   { apply Int24.mul_commut. }
   { apply Int32.mul_commut. }
+  { apply Int40.mul_commut. }
   { apply Int48.mul_commut. }
   { apply Int56.mul_commut. }
   { apply Int64.mul_commut. }
@@ -732,6 +761,7 @@ Proof.
   { rewrite Int16.eq_sym. reflexivity. }
   { rewrite Int24.eq_sym. reflexivity. }
   { rewrite Int32.eq_sym. reflexivity. }
+  { rewrite Int40.eq_sym. reflexivity. }
   { rewrite Int48.eq_sym. reflexivity. }
   { rewrite Int56.eq_sym. reflexivity. }
   { rewrite Int64.eq_sym. reflexivity. }
@@ -751,6 +781,7 @@ Proof.
   { apply Int16.and_commut. }
   { apply Int24.and_commut. }
   { apply Int32.and_commut. }
+  { apply Int40.and_commut. }
   { apply Int48.and_commut. }
   { apply Int56.and_commut. }
   { apply Int64.and_commut. }
@@ -770,6 +801,7 @@ Proof.
   { apply Int16.or_commut. }
   { apply Int24.or_commut. }
   { apply Int32.or_commut. }
+  { apply Int40.or_commut. }
   { apply Int48.or_commut. }
   { apply Int56.or_commut. }
   { apply Int64.or_commut. }
@@ -789,6 +821,7 @@ Proof.
   { apply Int16.xor_commut. }
   { apply Int24.xor_commut. }
   { apply Int32.xor_commut. }
+  { apply Int40.xor_commut. }
   { apply Int48.xor_commut. }
   { apply Int56.xor_commut. }
   { apply Int64.xor_commut. }
@@ -980,6 +1013,10 @@ Proof.
   }
   {
     remember (Int32.eq (smt_eval_ast m Sort_BV32 ast1) (smt_eval_ast m Sort_BV32 ast2)) as b.
+    destruct b; reflexivity.
+  }
+  {
+    remember (Int40.eq (smt_eval_ast m Sort_BV40 ast1) (smt_eval_ast m Sort_BV40 ast2)) as b.
     destruct b; reflexivity.
   }
   {
@@ -1444,6 +1481,7 @@ Definition sort_to_add s : (smt_sort_to_int_type s) -> (smt_sort_to_int_type s) 
   | Sort_BV16 => Int16.add
   | Sort_BV24 => Int24.add
   | Sort_BV32 => Int32.add
+  | Sort_BV40 => Int40.add
   | Sort_BV48 => Int48.add
   | Sort_BV56 => Int56.add
   | Sort_BV64 => Int64.add
@@ -1457,6 +1495,7 @@ Definition sort_to_sub s : (smt_sort_to_int_type s) -> (smt_sort_to_int_type s) 
   | Sort_BV16 => Int16.sub
   | Sort_BV24 => Int24.sub
   | Sort_BV32 => Int32.sub
+  | Sort_BV40 => Int40.sub
   | Sort_BV48 => Int48.sub
   | Sort_BV56 => Int56.sub
   | Sort_BV64 => Int64.sub
@@ -1470,6 +1509,7 @@ Definition sort_to_mul s : (smt_sort_to_int_type s) -> (smt_sort_to_int_type s) 
   | Sort_BV16 => Int16.mul
   | Sort_BV24 => Int24.mul
   | Sort_BV32 => Int32.mul
+  | Sort_BV40 => Int40.mul
   | Sort_BV48 => Int48.mul
   | Sort_BV56 => Int56.mul
   | Sort_BV64 => Int64.mul
@@ -1483,6 +1523,7 @@ Definition sort_to_udiv s : (smt_sort_to_int_type s) -> (smt_sort_to_int_type s)
   | Sort_BV16 => Int16.divu
   | Sort_BV24 => Int24.divu
   | Sort_BV32 => Int32.divu
+  | Sort_BV40 => Int40.divu
   | Sort_BV48 => Int48.divu
   | Sort_BV56 => Int56.divu
   | Sort_BV64 => Int64.divu
@@ -1496,6 +1537,7 @@ Definition sort_to_sdiv s : (smt_sort_to_int_type s) -> (smt_sort_to_int_type s)
   | Sort_BV16 => Int16.divs
   | Sort_BV24 => Int24.divs
   | Sort_BV32 => Int32.divs
+  | Sort_BV40 => Int40.divs
   | Sort_BV48 => Int48.divs
   | Sort_BV56 => Int56.divs
   | Sort_BV64 => Int64.divs
@@ -1509,6 +1551,7 @@ Definition sort_to_urem s : (smt_sort_to_int_type s) -> (smt_sort_to_int_type s)
   | Sort_BV16 => Int16.modu
   | Sort_BV24 => Int24.modu
   | Sort_BV32 => Int32.modu
+  | Sort_BV40 => Int40.modu
   | Sort_BV48 => Int48.modu
   | Sort_BV56 => Int56.modu
   | Sort_BV64 => Int64.modu
@@ -1522,6 +1565,7 @@ Definition sort_to_srem s : (smt_sort_to_int_type s) -> (smt_sort_to_int_type s)
   | Sort_BV16 => Int16.mods
   | Sort_BV24 => Int24.mods
   | Sort_BV32 => Int32.mods
+  | Sort_BV40 => Int40.mods
   | Sort_BV48 => Int48.mods
   | Sort_BV56 => Int56.mods
   | Sort_BV64 => Int64.mods
@@ -1535,6 +1579,7 @@ Definition sort_to_xor s : (smt_sort_to_int_type s) -> (smt_sort_to_int_type s) 
   | Sort_BV16 => Int16.xor
   | Sort_BV24 => Int24.xor
   | Sort_BV32 => Int32.xor
+  | Sort_BV40 => Int40.xor
   | Sort_BV48 => Int48.xor
   | Sort_BV56 => Int56.xor
   | Sort_BV64 => Int64.xor
@@ -1547,6 +1592,7 @@ Definition sort_to_shl s : (smt_sort_to_int_type s) -> (smt_sort_to_int_type s) 
   | Sort_BV16 => Int16.shl
   | Sort_BV24 => Int24.shl
   | Sort_BV32 => Int32.shl
+  | Sort_BV40 => Int40.shl
   | Sort_BV48 => Int48.shl
   | Sort_BV56 => Int56.shl
   | Sort_BV64 => Int64.shl
@@ -1560,6 +1606,7 @@ Definition sort_to_lshr s : (smt_sort_to_int_type s) -> (smt_sort_to_int_type s)
   | Sort_BV16 => Int16.shru
   | Sort_BV24 => Int24.shru
   | Sort_BV32 => Int32.shru
+  | Sort_BV40 => Int40.shru
   | Sort_BV48 => Int48.shru
   | Sort_BV56 => Int56.shru
   | Sort_BV64 => Int64.shru
@@ -1573,6 +1620,7 @@ Definition sort_to_ashr s : (smt_sort_to_int_type s) -> (smt_sort_to_int_type s)
   | Sort_BV16 => Int16.shr
   | Sort_BV24 => Int24.shr
   | Sort_BV32 => Int32.shr
+  | Sort_BV40 => Int40.shr
   | Sort_BV48 => Int48.shr
   | Sort_BV56 => Int56.shr
   | Sort_BV64 => Int64.shr
@@ -1586,6 +1634,7 @@ Definition sort_to_and s : (smt_sort_to_int_type s) -> (smt_sort_to_int_type s) 
   | Sort_BV16 => Int16.and
   | Sort_BV24 => Int24.and
   | Sort_BV32 => Int32.and
+  | Sort_BV40 => Int40.and
   | Sort_BV48 => Int48.and
   | Sort_BV56 => Int56.and
   | Sort_BV64 => Int64.and
@@ -1599,6 +1648,7 @@ Definition sort_to_or s : (smt_sort_to_int_type s) -> (smt_sort_to_int_type s) -
   | Sort_BV16 => Int16.or
   | Sort_BV24 => Int24.or
   | Sort_BV32 => Int32.or
+  | Sort_BV40 => Int40.or
   | Sort_BV48 => Int48.or
   | Sort_BV56 => Int56.or
   | Sort_BV64 => Int64.or
@@ -2032,6 +2082,7 @@ Proof.
   { apply equiv_smt_expr_refl. }
   { apply equiv_smt_expr_refl. }
   { apply equiv_smt_expr_refl. }
+  { apply equiv_smt_expr_refl. }
 Qed.
 
 Lemma equiv_smt_expr_simplify_cmpop_bv1 : forall op (ast1 ast2 : smt_ast Sort_BV1),
@@ -2170,6 +2221,7 @@ Proof.
   { apply equiv_smt_expr_refl. }
   { apply equiv_smt_expr_refl. }
   { apply equiv_smt_expr_simplify_cmpop_bv32. }
+  { apply equiv_smt_expr_refl. }
   { apply equiv_smt_expr_refl. }
   { apply equiv_smt_expr_refl. }
   { apply equiv_smt_expr_simplify_cmpop_bv64. }
